

$$dy/dx + p(x)y = Q(x)$$

$$p(x) = e^{\int P(x) dx}$$

$$y' + 2x^{-1}y = e^{3x}x^{-2}$$

$$p(x) = e^{\int 2x^{-1}} = e^{2\ln|x|} = x^2$$

$$y(x) = \frac{1}{p(x)} \int p(x) Q(x) dx$$

$$= \frac{1}{x^2} \int e^{3x} dx = \frac{e^{3x}}{3x^2} + \frac{C}{x^2}$$

The general solution to $x^2y' + 2xy = e^{3x}$ is

☐ A $y = \frac{3}{x^2}e^{3x} + C$

☒ B $y = Ce^{3x}$

☐ C $y = \frac{1}{3x^2}e^{3x} + Cx^{-2}$

☐ D $y = \frac{1}{2x^2}e^{3x}$

☐ E $y = \frac{1}{3x}e^{3x} + Cx^{-2}$

$$p(x) = e^{\int 3 dx} = e^{3x}$$

$$y(x) = \frac{1}{p(x)} \int Q(x) p(x) dx$$

$$= e^{-3x} \int 3x^2 + 2x dx$$

$$= e^{-3x} x^3 + e^{-3x} x + C e^{-3x}$$

Find a general solution to the following differential equation

$$\frac{dy}{dx} + 3y = 3x^2 e^{-3x} + 2x e^{-3x}$$

(A) $y = (x^3 + x^2) e^{-3x} + C$

(B) $y = (x^3 + x^2 + C) e^{-3x}$

(C) $y = (3x^2 + 2x + C) e^{-3x}$

(D) $y = -\left(x^2 + \frac{4}{3}x + \frac{4}{9}\right) e^{-3x} + C$

(E) $y = (x^3 + x^2) e^{-3x} + C e^{3x}$

$$y' - 3x^{-1}y = 2x^3$$

$$p(x) = e^{\int -3x^{-1} dx} = e^{-3 \ln x} = x^{-3}$$

$$y(x) = x^3 \int 2 dx = (2x + C)x^3$$

$$y(x) = 2x^4 + Cx^3$$

$$y(1) = 0 = 2 + C \rightarrow C = -2$$

$$y(2) = 32 - 16 = 16$$

Let $y(x)$ be the solution to the initial value problem

$$xy' = 3y + 2x^4, \quad y(1) = 0.$$

Then, $y(2)$ is

(A) 8

(B) 4

(C) 20

(D) 16

(E) 32

$$y' + \frac{y}{2+2x} = 6$$

$$p = e^{\int \frac{1}{2+2x} dx} = e^{\int \frac{1}{2} u^{-1} du} = e^{\frac{1}{2} \ln u}$$

$$u = 2+2x$$

$$\frac{du}{dx} = 2$$

$$dx = \frac{1}{2} du$$

$$= e^{\frac{1}{2} \ln(2+2x)}$$

$$= e^{\ln((2+2x)^{1/2})}$$

$$= (2+2x)^{1/2}$$

$$y(x) = \frac{1}{p(x)} \int Q(x) p(x) dx$$

$$= \frac{1}{(2+2x)^{1/2}} \int 6(2+2x)^{1/2} dx$$

$$u = 2+2x$$

$$dx = \frac{1}{2} du$$

$$= (2+2x)^{-1/2} \int 3 u^{1/2} dx = (2+2x)^{-1/2} \left[2 u^{3/2} + C \right]$$

$$= (2+2x)^{-1/2} \left[2(2+2x)^{3/2} + C \right]$$

$$y(x) = 2(2+2x) + C(2+2x)^{-1/2}$$

$$y(0) = 2 = 2(2+2(0)) + C(2+2(0))^{-1/2}$$

$$2 = 4 + \frac{C}{\sqrt{2}}$$

$$2\sqrt{2} = 4\sqrt{2} + C \rightarrow C = -2\sqrt{2}$$

$$y(3) = 2(2+2(3)) + (2+2(3))^{-1/2} (-2\sqrt{2})$$

$$= 16 + \frac{1}{2\sqrt{2}} (-2\sqrt{2}) = 15$$

If $y(x)$ is a solution to the initial value problem

$$\frac{dy}{dx} + \frac{y}{2+2x} = 6, \quad y(0) = 2$$

then $y(3) = ?$

(A) 12

(B) -17

(C) 28

(D) 15

(E) -23

$$\frac{dy}{dx} + p(x)y = Q(x)y^n$$

$$v = y^{1-n}$$

$$v = y^{1-n} = y^{-1}$$

$$\frac{dv}{dx} = -y^{-2} \frac{dy}{dx}$$

$$\frac{dy}{dx} y^{-2} + 4x^{-1} y^{-1} = 3$$

$$-\frac{dv}{dx} + 4x^{-1}v = 3 \rightarrow \frac{dv}{dx} - 4x^{-1}v = -3$$

$$\rho(x) = e^{\int -4x^{-1} dx} = e^{-4 \ln x} = e^{\ln(x^{-4})} = x^{-4}$$

$$v(x) = \frac{1}{\rho(x)} \int Q(x) \rho(x) dx$$

$$v(x) = x^4 \int -3x^{-4} dx = (x^{-3} + C)x^4$$

$$v(x) = x + Cx^4$$

$$y^{-1} = x + Cx^4$$

$$y(x) = \frac{1}{x + Cx^4}$$

$$y(1) = \frac{1}{2} = \frac{1}{1+C} \rightarrow C=1$$

$$y(2) = \frac{1}{2+16} = \frac{1}{18}$$

If y is a solution to the initial value problem for a Bernoulli equation

$$\frac{dy}{dx} + \frac{4y}{x} = 3y^2, \quad y(1) = \frac{1}{2},$$

then $y(2) = ?$ Hint: Use the substitution $v = y^{-1}$.

☒ (A) $\frac{1}{18}$

☐ (B) $\frac{1}{34}$

☐ (C) $\frac{1}{10}$

☐ (D) $\frac{1}{20}$

☐ (E) $\frac{1}{32}$

$$y' + \frac{4t}{t^2+1} y = \frac{1}{t^2+1}$$

$$\rho(t) = e^{\int \frac{4t}{t^2+1} dt} = e^{\int \frac{4}{u} \frac{1}{2} du} = \int \frac{2}{u} du$$

$$u = t^2 + 1$$

$$du/dt = 2t$$

$$dt = \frac{1}{2t} du$$

$$= e^{2 \ln u} = e^{\ln u^2} = u^2 = (t^2+1)^2$$

$$y(x) = \frac{1}{\rho(t)} \int Q(t) \rho(t) dt$$

$$= \frac{1}{(t^2+1)^2} \int (t^2+1)^2 \frac{1}{t^2+1} dt$$

$$= \frac{1}{(t^2+1)^2} \int t^2+1 dt = \frac{1}{(t^2+1)^2} \left[\frac{1}{3} t^3 + t + C \right]$$

Find the general solution of the equation

$$(t^2 + 1) \frac{dy}{dt} + 4ty = 1$$

(A) $y = \frac{\frac{1}{2}t^2 + C}{t^2 + 1}$

(B) $y = (t^2 + 1)(\tan^{-1}(t) + C)$

(C) $y = e^{-4t}(\tan^{-1}(t) + C)$

(D) $y = \frac{\frac{1}{3}t^3 + t + C}{(t^2 + 1)^2}$

(E) $y = 2 \ln(t^2 + 1) + C$

$$F = -mg - \frac{1}{25}v$$

$$F = ma = m \frac{dv}{dt}$$

$$-mg - \frac{1}{25}v = m \frac{dv}{dt}$$

$$-0.2(9.8) - \frac{v}{25} = 0.2 \frac{dv}{dt}$$

$$-\frac{1}{5} \frac{dv}{dt} - \frac{v}{25} = \frac{1}{5}(9.8)$$

$$\frac{dv}{dt} + \frac{1}{5}v = -9.8$$

$$\textcircled{1} \quad y' + p(x)y = Q(x)$$

$$\textcircled{2} \quad \rho(x) = e^{\int p(x) dx}$$

$$\textcircled{3} \quad y(x) = \frac{1}{\rho(x)} \int Q(x) \rho(x) dx$$

$$\rho(t) = e^{\int \frac{1}{5} dt} = e^{\frac{1}{5}t}$$

$$v(t) = e^{-\frac{1}{5}t} \int -9.8 e^{\frac{1}{5}t} dt = e^{-\frac{1}{5}t} \left[-49 e^{\frac{1}{5}t} + C \right]$$

$$v(t) = -49 + C e^{-\frac{1}{5}t}$$

$$v(0) = -49 + C e^0 = 49 \rightarrow C = 98$$

$$v(t) = -49 + 98 e^{-\frac{t}{5}}$$

$$0 = -49 + 98 e^{-\frac{t}{5}}$$

$$\frac{1}{2} = e^{-\frac{t}{5}}$$

$$\ln \frac{1}{2} = -\frac{t}{5}$$

$$t = -5 \ln \frac{1}{2} = -5(\ln 1 - \ln 2) = 5 \ln 2 = \ln 32$$

A ball with mass 0.2 kg is thrown upward with initial velocity 49 m/s from the ground. There is a force due to air resistance of magnitude $|v|/25$ directed opposite to the velocity v (measured in m/s). How much time does it take for the ball to reach its maximum height? (Use that the gravitation acceleration $g = 9.8 \text{ m/s}^2$.)

$$W(f, g) = \det \begin{vmatrix} f(t) & g(t) \\ f'(t) & g'(t) \end{vmatrix}$$

$$4t^4 = \det \begin{vmatrix} t^2 & g(t) \\ 2t & g'(t) \end{vmatrix} = t^2 g' - 2tg$$

$$t^2 g' - 2tg = 4t^4$$

$$g' - 2t^{-1}g = 4t^2$$

$y' + p(x)y = Q(x) \rightarrow$ easy to solve with integrating factor

$$p(t) = e^{\int -2t^{-1} dt} = e^{-2 \ln t} = t^{-2}$$

$$g(t) = t^2 \int (4t^2)(t^{-2}) dt = t^2 [4t + C] = 4t^3 + Ct^2$$

If the Wronskian $W(f, g) = 4t^4$ and $f(t) = t^2$, for $t > 0$, then the function g could be:

(A) $Ct + 4t^4$

(B) $Ct^2 + 4t^2$

(C) $Ct^2 + 4t^4$

(D) $Ct + 4t^3$

(E) $Ct^2 + 4t^3$

$$y' - x^{-1}y = x^3$$

$$\rho(x) = e^{\int -x^{-1} dx} = e^{-\ln x} = x^{-1}$$

$$y(x) = x \int x^2 dx = x \left[\frac{1}{3} x^3 + C \right] = \frac{x^4}{3} + Cx$$

$$y(1) = \frac{1}{3} + C = \frac{4}{3} \rightarrow C = 1$$

$$y(3) = \frac{3^4}{3} + 3 = 3^3 + 3 = 30$$

If y is a solution to the the initial value problem

$$\frac{dy}{dx} - \frac{y}{x} = x^3, \quad y(1) = \frac{4}{3}$$

then $y(3) = ?$

(A) 20

(B) 4

(C) 27

☒ (D) 30

(E) $\frac{8}{3}$

$$y' + 5x^{-1}y = e^{4x}x^{-5}$$

$$p(x) = e^{\int 5x^{-1} dx} = e^{5 \ln x} = x^5$$

$$y(x) = x^{-5} \int e^{4x} dx$$

$$= x^{-5} \left[\frac{1}{4} e^{4x} + C \right]$$

The general solution $y(x)$ to

$$x^2 y' + 5xy = \frac{e^{4x}}{x^3}, \quad x > 0$$

is

(A) $y(x) = \frac{e^{4x}}{x^3} + C$

(B) $y(x) = \frac{e^{4x}}{4x^5} + \frac{C}{x^5}$

(C) $y(x) = \frac{e^x}{x^3} + \frac{C}{x^3}$

(D) $y(x) = Cx^{-5}$

(E) $y(x) = \frac{Ce^{4x}}{4}$

$$y' + 2e^{-x}y = 2e^{2e^{-x}}$$

$$p(x) = e^{\int 2e^{-x} dx} = e^{-2e^{-x}}$$

$$y(x) = e^{2e^{-x}} \int 2 dx$$

$$e^{2e^{-x}} [2x + C]$$

$$y(x) = 2xe^{2e^{-x}} + Ce^{2e^{-x}}$$

Find the general solution to the differential equation

$$e^x \frac{dy}{dx} + 2y = 2e^{x+2e^{-x}}.$$

(A) $y = x^2 e^{2e^{-x}} + C e^{2e^{-x}}$

(B) $y = x e^{x+2e^{-x}} + C e^{x+2e^{-x}}$

(C) $y = x^2 e^x + C e^x$

(D) $y = x^2 e^{-x} + C e^{x+2e^{-x}}$

(E) $y = 2x e^{2e^{-x}} + C e^{2e^{-x}}$